Implement some more of enum parsing

examples/kv_parsing/EnumParsing.fst
@@ -3,6 +3,10 @@ module EnumParsing
 open PureParser
 open Validator
 open Serializer
+open Slice
+
+open FStar.HyperStack
+open FStar.HyperStack.ST
 
 module U8 = FStar.UInt8
 module U16 = FStar.UInt16
@@ -35,7 +39,7 @@ let parse_numbers_tag : parser numbers_tag =
   (fun t -> if U8.lt t 3uy then parse_ret (t <: numbers_tag) else fail_parser)
 
 let parse_Nothing : parser (ns:numbers{Nothing? ns}) =
-  parse_ret #(ns:numbers{Nothing? ns}) Nothing
+  parse_ret Nothing
 
 let parse_OneNum : parser (ns:numbers{OneNum? ns}) =
   parse_u32 `and_then`
@@ -57,3 +61,44 @@ let parse_numbers : parser numbers =
             assert (U8.v t == 2);
             parse_TwoNums `and_then` parse_ret
            end)
+
+let parse_numbers_tag_st : parser_st parse_numbers_tag = fun input ->
+  match parse_u8_st input with
+  | Some (tag, off) -> if U8.lt tag 3uy
+                      then Some ((tag <: numbers_tag), off)
+                      else None
+  | None -> None
+
+let parse_numbers_tag_st_nochk : parser_st_nochk parse_numbers_tag = fun input ->
+  let (tag, off) = parse_u8_st_nochk input in
+  ((tag <: numbers_tag), off)
+
+let check_length (len:U32.t) (input:bslice) : Pure bool
+  (requires True)
+  (ensures (fun r -> r ==> U32.v input.len >= U32.v len)) = U32.lte len input.len
+
+val validate_OneNum : stateful_validator parse_OneNum
+let validate_OneNum = fun input ->
+  if check_length 4ul input then Some 4ul else None
+
+val validate_TwoNums : stateful_validator parse_TwoNums
+let validate_TwoNums = fun input ->
+  if check_length 8ul input then Some 8ul else None
+
+#reset-options "--z3rlimit 10"
+
+let validate_numbers : stateful_validator parse_numbers = fun input ->
+  match parse_numbers_tag_st input with
+  | Some (tag, off) -> if U8.eq tag 0uy
+                        then Some off
+                      else if U8.eq tag 1uy
+                        then match validate_OneNum (advance_slice input off) with
+                             | Some off' -> if u32_add_overflows off off' then None else Some (U32.add off off')
+                             | None -> None
+                      else begin
+                             assert (U8.v tag == 2);
+                             match validate_TwoNums (advance_slice input off) with
+                             | Some off' -> if u32_add_overflows off off' then None else Some (U32.add off off')
+                             | None -> None
+                           end
+  | None -> None
